some bviProps

compiler1/semantics/bviPropsScript.sml
@@ -57,4 +57,78 @@ val evaluate_SNOC = store_thm("evaluate_SNOC",
   \\ Cases_on `a''` \\ fs [LENGTH]
   \\ REV_FULL_SIMP_TAC std_ss [LENGTH_NIL] \\ fs []);
 
+val inc_clock_def = Define `
+  inc_clock n (s:bviSem$state) = s with clock := s.clock + n`;
+
+val inc_clock_ZERO = store_thm("inc_clock_ZERO",
+  ``!s. inc_clock 0 s = s``,
+  fs [inc_clock_def,state_component_equality]);
+
+val inc_clock_ADD = store_thm("inc_clock_ADD",
+  ``inc_clock n (inc_clock m s) = inc_clock (n+m) s``,
+  fs [inc_clock_def,state_component_equality,AC ADD_ASSOC ADD_COMM]);
+
+val dec_clock_inv_clock = store_thm("dec_clock_inv_clock",
+  ``¬(t1.clock < ticks + 1) ==>
+    (dec_clock (ticks + 1) (inc_clock c t1) = inc_clock c (dec_clock (ticks + 1) t1))``,
+  fs [dec_clock_def,inc_clock_def,state_component_equality] \\ DECIDE_TAC);
+
+val dec_clock_inv_clock1 = store_thm("dec_clock_inv_clock1",
+  ``t1.clock <> 0 ==>
+    (dec_clock 1 (inc_clock c t1) = inc_clock c (dec_clock 1 t1))``,
+  fs [dec_clock_def,inc_clock_def,state_component_equality] \\ DECIDE_TAC);
+
+val do_app_inv_clock = prove(
+  ``case do_app op (REVERSE a) s of
+    | Rerr e => (do_app op (REVERSE a) (inc_clock n s) = Rerr e)
+    | Rval (v,s1) => (do_app op (REVERSE a) (inc_clock n s) = Rval (v,inc_clock n s1))``,
+  fs [bviSemTheory.do_app_def] \\ Cases_on `op` \\ fs [do_app_aux_def,bvlSemTheory.do_app_def]
+  \\ BasicProvers.EVERY_CASE_TAC
+  \\ fs [bvi_to_bvl_def,closSemTheory.get_global_def,inc_clock_def,bvl_to_bvi_def,LET_DEF]
+  \\ SRW_TAC [] [] \\ REV_FULL_SIMP_TAC std_ss []);
+
+val evaluate_inv_clock = store_thm("evaluate_inv_clock",
+  ``!xs env t1 res t2 n.
+      (evaluate (xs,env,t1) = (res,t2)) /\ res <> Rerr(Rabort Rtimeout_error) ==>
+      (evaluate (xs,env,inc_clock n t1) = (res,inc_clock n t2))``,
+  SIMP_TAC std_ss [] \\ recInduct evaluate_ind \\ REPEAT STRIP_TAC
+  \\ fs [evaluate_def]
+  THEN1 (`?res5 s5. evaluate ([x],env,s) = (res5,s5)` by METIS_TAC [PAIR]
+    \\ `?res6 s6. evaluate (y::xs,env,s5) = (res6,s6)` by METIS_TAC [PAIR]
+    \\ fs [] \\ REVERSE (Cases_on `res5`) \\ fs [] \\ SRW_TAC [] []
+    \\ Cases_on `res6` \\ fs [] \\ SRW_TAC [] []
+    \\ Cases_on`e` \\ fs[])
+  THEN1 (Cases_on `n < LENGTH env` \\ fs [] \\ SRW_TAC [] [])
+  \\ TRY (`?res5 s5. evaluate ([x1],env,s) = (res5,s5)` by METIS_TAC [PAIR]
+    \\ fs [] \\ Cases_on `res5` \\ fs [] \\ SRW_TAC [] [] \\ fs [] \\ NO_TAC)
+  THEN1 (`?res5 s5. evaluate (xs,env,s) = (res5,s5)` by METIS_TAC [PAIR]
+    \\ fs [] \\ Cases_on `res5` \\ fs [] \\ SRW_TAC [] []
+    \\ Cases_on`e` \\ fs[])
+  \\ TRY (Cases_on `s.clock = 0` \\ fs []
+    \\ `(inc_clock n s).clock <> 0` by (EVAL_TAC \\ DECIDE_TAC)
+    \\ fs [dec_clock_inv_clock1] \\ NO_TAC)
+  THEN1
+   (`?res5 s5. evaluate (xs,env,s) = (res5,s5)` by METIS_TAC [PAIR]
+    \\ fs [] \\ Cases_on `res5` \\ fs [] \\ SRW_TAC [] []
+    \\ TRY (Cases_on`e` \\ fs[] \\ NO_TAC)
+    \\ MP_TAC (do_app_inv_clock |> Q.INST [`s`|->`s5`])
+    \\ Cases_on `do_app op (REVERSE a) s5` \\ fs [] \\ SRW_TAC [] []
+    \\ Cases_on `a'` \\ fs [] \\ SRW_TAC [] [])
+  THEN1
+   (Cases_on `dest = NONE /\ IS_SOME handler` \\ fs []
+    \\ Cases_on `evaluate (xs,env,s1)` \\ fs []
+    \\ Cases_on `q` \\ fs []
+    \\ `(inc_clock n r).code = r.code` by SRW_TAC [] [inc_clock_def] \\ fs []
+    \\ Cases_on `find_code dest a r.code` \\ fs [] \\ SRW_TAC [] []
+    \\ TRY (Cases_on`e` \\ fs[] \\ NO_TAC)
+    \\ Cases_on `x` \\ fs []
+    \\ Cases_on `r.clock < ticks + 1` \\ fs [] \\ SRW_TAC [] []
+    \\ IMP_RES_TAC dec_clock_inv_clock
+    \\ POP_ASSUM (ASSUME_TAC o GSYM)
+    \\ Cases_on `evaluate ([r'],q,dec_clock (ticks + 1) r)` \\ fs []
+    \\ Cases_on `q'` \\ fs [] \\ SRW_TAC [] []
+    \\ TRY(Cases_on`e` \\ fs[] \\ Cases_on`a'` \\ fs[] \\ rw[])
+    \\ RES_TAC \\ TRY (fs [inc_clock_def] \\ decide_tac)
+    \\ Cases_on `handler` \\ fs [] \\ rw[]));
+
 val _ = export_theory();
